Code cleanup: isolated RG material from coresem, forward-simulations etc into separate files, in preparation of the RG-free material to be released in VST1.0/book/paper

sepcomp/forward_simulations.v
@@ -12,6 +12,18 @@ Require Import Axioms.
 Require Import sepcomp.mem_lemmas. (*needed for definition of mem_forward etc*)
 Require Import sepcomp.core_semantics.
 
+Lemma external_call_mem_forward:
+  forall (ef : external_function) (F V : Type) (ge : Genv.t F V)
+    (vargs : list val) (m1 : mem) (t : trace) (vres : val) (m2 : mem),
+    external_call ef ge vargs m1 t vres m2 -> mem_forward m1 m2.
+Proof.
+intros.
+intros b Hb.
+split; intros. eapply external_call_valid_block; eauto.
+eapply external_call_max_perm; eauto.
+Qed.
+
+
 Definition val_inject_opt (j: meminj) (v1 v2: option val) :=
   match v1, v2 with Some v1', Some v2' => val_inject j v1' v2'
   | None, None => True
@@ -96,27 +108,38 @@ Module Forward_simulation_eq. Section Forward_simulation_equals.
 End Forward_simulation_equals. 
 
 (*Question: Does this declaration take effect after module import?*)
-Implicit Arguments Forward_simulation_equals [[G1] [C1] [G2] [C2]]. 
+Implicit Arguments Forward_simulation_equals [[M] [G1] [C1] [G2] [C2]]. 
 
 End Forward_simulation_eq.
 
 (** * Next, an axiom for passes that allow the memory to undergo extension. *)
+(*As extensions require CompCert memories, such simulations can only be formulated 
+for core semantics with (M:=mem)*)
 
 Module Forward_simulation_ext. Section Forward_simulation_extends. 
   Context {G1 C1 G2 C2:Type}
-          {Sem1: RelyGuaranteeSemantics G1 C1}
-          {Sem2: RelyGuaranteeSemantics  G2 C2}
+          {Sem1 : CoreSemantics G1 C1 mem}
+          {Sem2 : CoreSemantics G2 C2 mem}
 
           {ge1:G1}
           {ge2:G2}
           {entry_points : list (val * val * signature)}.
 
-  Record Forward_simulation_extends := 
+  Record Forward_simulation_extends :=
   { core_data : Type;
 
     match_state : core_data -> C1 -> mem -> C2 -> mem -> Prop;
     core_ord : core_data -> core_data -> Prop;
     core_ord_wf : well_founded core_ord;
+
+    (*Matching memories should be well-defined ie not contain values
+        with invalid/"dangling" block numbers*)
+    match_memwd: forall d c1 m1 c2 m2,  match_state d c1 m1 c2 m2 -> 
+      (mem_wd m1 /\ mem_wd m2);
+
+    (*The following axiom could be strengthened to extends m1 m2*)
+    match_validblocks: forall d c1 m1 c2 m2,  match_state d c1 m1 c2 m2 -> 
+      forall b, Mem.valid_block m1 b <-> Mem.valid_block m2 b;
 
     core_diagram : 
       forall st1 m1 st1' m1', corestep Sem1 ge1 st1 m1 st1' m1' ->
@@ -124,11 +147,6 @@ Module Forward_simulation_ext. Section Forward_simulation_extends.
         match_state cd st1 m1 st2 m2 ->
         exists st2', exists m2', exists cd',
           match_state cd' st1' m1' st2' m2' /\
-          Mem.unchanged_on (fun b ofs => 
-            (*I'm not sure whether this should be ~private_block st1 or
-               ~private_block st2.  Perhaps it doesn't matter if we know that 
-               private_block st2 -> private_block st1 over extension passes. *)
-            loc_out_of_bounds m1 b ofs /\ ~private_block Sem1 st1 b) m2 m2' /\
           ((corestep_plus Sem2 ge2 st2 m2 st2' m2') \/
             corestep_star Sem2 ge2 st2 m2 st2' m2' /\
             core_ord cd' cd);
@@ -139,6 +157,7 @@ Module Forward_simulation_ext. Section Forward_simulation_extends.
           Forall2 Val.lessdef vals vals' ->
           Forall2 (Val.has_type) vals' (sig_args sig) ->
           Mem.extends m1 m2 ->
+          mem_wd m1 -> mem_wd m2 ->
           exists cd, exists c1, exists c2,
             initial_core Sem1 ge1 v1 vals = Some c1 /\
             initial_core Sem2 ge2 v2 vals' = Some c2 /\
@@ -147,25 +166,28 @@ Module Forward_simulation_ext. Section Forward_simulation_extends.
     core_halted : 
       forall cd st1 m1 st2 m2 v1,
         match_state cd st1 m1 st2 m2 ->
-        halted Sem1 st1 = Some v1 ->
+        halted Sem1 st1 = Some v1 -> val_valid v1 m1 ->
         exists v2, Val.lessdef v1 v2 /\
             halted Sem2 st2 = Some v2 /\
-            Mem.extends m1 m2;
+            Mem.extends m1 m2 /\ val_valid v2 m2;
 
     core_at_external : 
       forall cd st1 m1 st2 m2 e vals1 ef_sig,
         match_state cd st1 m1 st2 m2 ->
         at_external Sem1 st1 = Some (e,ef_sig,vals1) ->
+        (forall v1, In v1 vals1 -> val_valid v1 m1) -> 
         exists vals2,
           Mem.extends m1 m2 /\
           Forall2 Val.lessdef vals1 vals2 /\
           Forall2 (Val.has_type) vals2 (sig_args ef_sig) /\
-          at_external Sem2 st2 = Some (e,ef_sig,vals2);
+          at_external Sem2 st2 = Some (e,ef_sig,vals2) /\
+          (forall v2, In v2 vals2 -> val_valid v2 m2);
 
     core_after_external :
       forall cd st1 st2 m1 m2 e vals1 vals2 ret1 ret2 m1' m2' ef_sig,
         match_state cd st1 m1 st2 m2 ->
         at_external Sem1 st1 = Some (e,ef_sig,vals1) ->
+        (forall v1, In v1 vals1 -> val_valid v1 m1) -> 
         at_external Sem2 st2 = Some (e,ef_sig,vals2) ->
 
         Forall2 Val.lessdef vals1 vals2 ->
@@ -173,28 +195,29 @@ Module Forward_simulation_ext. Section Forward_simulation_extends.
         mem_forward m1 m1' ->
         mem_forward m2 m2' ->
 
-        Mem.unchanged_on (fun b ofs => 
-          loc_out_of_bounds m1 b ofs /\ private_block Sem1 st1 b) m2 m2' -> 
-       (*i.e., spill-locations didn't change*)
+        Mem.unchanged_on (loc_out_of_bounds m1) m2 m2' -> 
+        (*i.e., spill-locations didn't change*)
         Val.lessdef ret1 ret2 ->
         Mem.extends m1' m2' ->
 
         Val.has_type ret2 (proj_sig_res ef_sig) -> 
 
+        mem_wd m1' -> mem_wd m2' -> val_valid ret1 m1' -> val_valid ret2 m2' ->
+
         exists st1', exists st2', exists cd',
           after_external Sem1 (Some ret1) st1 = Some st1' /\
           after_external Sem2 (Some ret2) st2 = Some st2' /\
           match_state cd' st1' m1' st2' m2' }.
-
 End Forward_simulation_extends.
 
 Implicit Arguments Forward_simulation_extends [[G1] [C1] [G2] [C2]].
 
 End Forward_simulation_ext.
 
-(** Perhaps the "Coop" versions of each record should become the
-   standard versions everywhere? *)
-
+(*The same for CoopCoreSem's - but this can just be obtained by instantiating the
+previous definition to 
+          {Sem1 : CoopCoreSem G1 C1}
+          {Sem2 : CoopCoreSem G2 C2}
 Module Coop_forward_simulation_ext. Section Forward_simulation_extends. 
   Context {G1 C1 G2 C2:Type}
           {Sem1 : CoopCoreSem G1 C1}
@@ -292,101 +315,15 @@ End Forward_simulation_extends.
 Implicit Arguments Forward_simulation_extends [[G1] [C1] [G2] [C2]].
 
 End Coop_forward_simulation_ext.
+*)
 
 (** An axiom for passes that use memory injections. *)
+(*Again, we specialize (M:=mem), and also G1:=Genv F1 V1, due to
+the typing constraint of meminj_preserves_globals ge1 j
+in the at_external clause*)
+
 
 Module Forward_simulation_inj. Section Forward_simulation_inject. 
-  Context {F1 V1 C1 G2 C2:Type}
-          {Sem1 : RelyGuaranteeSemantics (Genv.t F1 V1) C1}
-          {Sem2 : RelyGuaranteeSemantics G2 C2}
-          {ge1: Genv.t F1 V1}
-          {ge2:G2}
-          {entry_points : list (val * val * signature)}.
-
-  Record Forward_simulation_inject := 
-  { core_data : Type;
-    match_state : core_data -> meminj -> C1 -> mem -> C2 -> mem -> Prop;
-    core_ord : core_data -> core_data -> Prop;
-    core_ord_wf : well_founded core_ord;
-    core_diagram : 
-      forall st1 m1 st1' m1', corestep Sem1 ge1 st1 m1 st1' m1' ->
-      forall cd st2 j m2,
-        match_state cd j st1 m1 st2 m2 ->
-        exists st2', exists m2', exists cd', exists j',
-          inject_incr j j' /\
-          inject_separated j j' m1 m2 /\
-          match_state cd' j' st1' m1' st2' m2' /\
-          Mem.unchanged_on (fun b ofs => 
-            loc_unmapped j b ofs /\ ~private_block Sem1 st1 b) m1 m1' /\
-          Mem.unchanged_on (fun b ofs => 
-            loc_out_of_reach j m1 b ofs /\ ~private_block Sem2 st2 b) m2 m2' /\
-          ((corestep_plus Sem2 ge2 st2 m2 st2' m2') \/
-            corestep_star Sem2 ge2 st2 m2 st2' m2' /\
-            core_ord cd' cd);
-
-    core_initial : forall v1 v2 sig,
-       In (v1,v2,sig) entry_points -> 
-       forall vals1 c1 m1 j vals2 m2,
-          initial_core Sem1 ge1 v1 vals1 = Some c1 ->
-          Mem.inject j m1 m2 -> 
-          Forall2 (val_inject j) vals1 vals2 ->
-          Forall2 (Val.has_type) vals2 (sig_args sig) ->
-          exists cd, exists c2, 
-            initial_core Sem2 ge2 v2 vals2 = Some c2 /\
-            match_state cd j c1 m1 c2 m2;
-
-    core_halted : forall cd j c1 m1 c2 m2 v1 rty,
-      match_state cd j c1 m1 c2 m2 ->
-      halted Sem1 c1 = Some v1 ->
-      Val.has_type v1 rty -> 
-      exists v2, val_inject j v1 v2 /\
-          halted Sem2 c2 = Some v2 /\
-          Val.has_type v2 rty /\
-          Mem.inject j m1 m2;
-
-    core_at_external : 
-      forall cd j st1 m1 st2 m2 e vals1 sig,
-        match_state cd j st1 m1 st2 m2 ->
-        at_external Sem1 st1 = Some (e,sig,vals1) ->
-        ( Mem.inject j m1 m2 /\
-          meminj_preserves_globals ge1 j /\ 
-          exists vals2, Forall2 (val_inject j) vals1 vals2 /\
-          Forall2 (Val.has_type) vals2 (sig_args (ef_sig e)) /\
-          at_external Sem2 st2 = Some (e,sig,vals2));
-
-    core_after_external :
-      forall cd j j' st1 st2 m1 e vals1 ret1 m1' m2 m2' ret2 sig,
-        Mem.inject j m1 m2->
-        match_state cd j st1 m1 st2 m2 ->
-        at_external Sem1 st1 = Some (e,sig,vals1) ->
-        meminj_preserves_globals ge1 j -> 
-
-        inject_incr j j' ->
-        inject_separated j j' m1 m2 ->
-        Mem.inject j' m1' m2' ->
-        val_inject_opt j' ret1 ret2 ->
-
-         mem_forward m1 m1'  -> 
-         Mem.unchanged_on (fun b ofs => 
-           loc_unmapped j b ofs /\ private_block Sem1 st1 b) m1 m1' ->
-         mem_forward m2 m2' -> 
-         Mem.unchanged_on (fun b ofs => 
-           loc_out_of_reach j m1 b ofs /\ private_block Sem2 st2 b) m2 m2' ->
-         val_has_type_opt' ret1 (proj_sig_res (ef_sig e)) -> 
-         val_has_type_opt' ret2 (proj_sig_res (ef_sig e)) -> 
-
-        exists cd', exists st1', exists st2',
-          after_external Sem1 ret1 st1 = Some st1' /\
-          after_external Sem2 ret2 st2 = Some st2' /\
-          match_state cd' j' st1' m1' st2' m2' }.
-
-End Forward_simulation_inject. 
-
-Implicit Arguments Forward_simulation_inject [[F1][V1] [C1] [G2] [C2]].
-
-End Forward_simulation_inj.
-
-Module Coop_forward_simulation_inj. Section Forward_simulation_inject. 
   Context {F1 V1 C1 G2 C2:Type}
           {Sem1 : CoreSemantics (Genv.t F1 V1) C1 mem}
           {Sem2 : CoreSemantics G2 C2 mem}
@@ -486,411 +423,26 @@ Module Coop_forward_simulation_inj. Section Forward_simulation_inject.
 
 End Forward_simulation_inject. 
 
-Implicit Arguments Forward_simulation_inject [[F1][V1] [C1] [G2] [C2]].
+Implicit Arguments Forward_simulation_inject [[F1] [V1] [C1] [G2] [C2]].
 
-End Coop_forward_simulation_inj.
+End Forward_simulation_inj.
 
-(* A variation of Forward_simulation_inj that exposes core_data and match_state *)
+Module Forward_simulation.
+Section Fwd_sim.
+Context {F1 V1 C1 F2 V2 C2:Type}
+        {Sem1 : CoreSemantics (Genv.t F1 V1) C1 mem}
+        {Sem2 : CoreSemantics (Genv.t F2 V2) C2 mem}.
 
-Module Forward_simulation_inj_exposed. Section Forward_simulation_inject. 
-  Context {F1 V1 C1 G2 C2:Type}
-          {Sem1 : RelyGuaranteeSemantics (Genv.t F1 V1) C1}
-          {Sem2 : RelyGuaranteeSemantics G2 C2}
+Inductive sim G1 G2 entrypoints:Type :=
+  sim_eq: forall (R:@Forward_simulation_eq.Forward_simulation_equals 
+                    mem _ _ _ _ Sem1 Sem2 G1 G2 entrypoints),
+          sim G1 G2 entrypoints
+| sim_ext: forall (R:@Forward_simulation_ext.Forward_simulation_extends
+                    _ _ _ _ Sem1 Sem2 G1 G2 entrypoints),
+          sim G1 G2 entrypoints
+| sim_inj: forall (R:@Forward_simulation_inj.Forward_simulation_inject
+                    _ _ _ _ _ Sem1 Sem2 G1 G2 entrypoints),
+          sim G1 G2 entrypoints.
+End Fwd_sim.
 
-          {ge1: Genv.t F1 V1}
-          {ge2:G2}
-          {entry_points : list (val * val * signature)}
-          {core_data : Type}
-          {match_state : core_data -> meminj -> C1 -> mem -> C2 -> mem -> Prop}
-          {core_ord : core_data -> core_data -> Prop}.
-
-  Record Forward_simulation_inject := 
-  { core_ord_wf : well_founded core_ord;
-    core_diagram : 
-      forall st1 m1 st1' m1', corestep Sem1 ge1 st1 m1 st1' m1' ->
-      forall cd st2 j m2,
-        match_state cd j st1 m1 st2 m2 ->
-        exists st2', exists m2', exists cd', exists j',
-          inject_incr j j' /\
-          inject_separated j j' m1 m2 /\
-          match_state cd' j' st1' m1' st2' m2' /\
-          Mem.unchanged_on (fun b ofs => 
-            loc_unmapped j b ofs /\ ~private_block Sem1 st1 b) m1 m1' /\
-          Mem.unchanged_on (fun b ofs => 
-            loc_out_of_reach j m1 b ofs /\ ~private_block Sem2 st2 b) m2 m2' /\
-          ((corestep_plus Sem2 ge2 st2 m2 st2' m2') \/
-            corestep_star Sem2 ge2 st2 m2 st2' m2' /\
-            core_ord cd' cd);
-
-    core_initial : forall v1 v2 sig,
-       In (v1,v2,sig) entry_points -> 
-       forall vals1 c1 m1 j vals2 m2,
-          initial_core Sem1 ge1 v1 vals1 = Some c1 ->
-          Mem.inject j m1 m2 -> 
-           Forall2 (val_inject j) vals1 vals2 ->
-          Forall2 (Val.has_type) vals2 (sig_args sig) ->
-          exists cd, exists c2, 
-            initial_core Sem2 ge2 v2 vals2 = Some c2 /\
-            match_state cd j c1 m1 c2 m2;
-
-    core_halted : forall cd j c1 m1 c2 m2 v1 rty,
-      match_state cd j c1 m1 c2 m2 ->
-      halted Sem1 c1 = Some v1 ->
-      Val.has_type v1 rty -> 
-      exists v2, val_inject j v1 v2 /\
-        halted Sem2 c2 = Some v2 /\
-        Val.has_type v2 rty /\
-        Mem.inject j m1 m2;
-
-    core_at_external : 
-      forall cd j st1 m1 st2 m2 e vals1 sig,
-        match_state cd j st1 m1 st2 m2 ->
-        at_external Sem1 st1 = Some (e,sig,vals1) ->
-        ( Mem.inject j m1 m2 /\
-          meminj_preserves_globals ge1 j /\ 
-          exists vals2, Forall2 (val_inject j) vals1 vals2 /\
-          Forall2 (Val.has_type) vals2 (sig_args (ef_sig e)) /\
-          at_external Sem2 st2 = Some (e,sig,vals2));
-
-    core_after_external :
-      forall cd j j' st1 st2 m1 e vals1 ret1 m1' m2 m2' ret2 sig,
-        Mem.inject j m1 m2->
-        match_state cd j st1 m1 st2 m2 ->
-        at_external Sem1 st1 = Some (e,sig,vals1) ->
-        meminj_preserves_globals ge1 j -> 
-
-        inject_incr j j' ->
-        inject_separated j j' m1 m2 ->
-        Mem.inject j' m1' m2' ->
-        val_inject_opt j' ret1 ret2 ->
-
-         mem_forward m1 m1'  -> 
-         Mem.unchanged_on (fun b ofs => 
-           loc_unmapped j b ofs /\ private_block Sem1 st1 b) m1 m1' ->
-         mem_forward m2 m2' -> 
-         Mem.unchanged_on (fun b ofs => 
-           loc_out_of_reach j m1 b ofs /\ private_block Sem2 st2 b) m2 m2' ->
-         val_has_type_opt' ret1 (proj_sig_res (ef_sig e)) -> 
-         val_has_type_opt' ret2 (proj_sig_res (ef_sig e)) -> 
-
-        exists cd', exists st1', exists st2',
-          after_external Sem1 ret1 st1 = Some st1' /\
-          after_external Sem2 ret2 st2 = Some st2' /\
-          match_state cd' j' st1' m1' st2' m2'
-    }.
-
-End Forward_simulation_inject. 
-
-Implicit Arguments Forward_simulation_inject [[F1][V1] [C1] [G2] [C2]].
-
-End Forward_simulation_inj_exposed.
-
-Lemma Forward_simulation_inj_exposed_hidden: 
-  forall (F1 V1 C1 G2 C2: Type) 
-   (csemS: RelyGuaranteeSemantics (Genv.t F1 V1) C1)
-   (csemT: RelyGuaranteeSemantics G2 C2) ge1 ge2 
-   entry_points core_data match_state core_ord,
-  Forward_simulation_inj_exposed.Forward_simulation_inject csemS csemT ge1 ge2
-    entry_points core_data match_state core_ord -> 
-  Forward_simulation_inj.Forward_simulation_inject csemS csemT ge1 ge2 entry_points.
-Proof.
-intros until core_ord; intros []; intros.
-solve[eapply @Forward_simulation_inj.Build_Forward_simulation_inject 
- with (core_data := core_data) (match_state := match_state); eauto].
-Qed.
-
-Lemma Forward_simulation_inj_hidden_exposed:
-  forall (F1 V1 C1 G2 C2: Type) 
-   (csemS: RelyGuaranteeSemantics (Genv.t F1 V1) C1)
-   (csemT: RelyGuaranteeSemantics G2 C2) ge1 ge2 entry_points,
-  Forward_simulation_inj.Forward_simulation_inject csemS csemT ge1 ge2 entry_points -> 
-  {core_data: Type & 
-  {match_state: core_data -> meminj -> C1 -> mem -> C2 -> mem -> Prop &
-  {core_ord: core_data -> core_data -> Prop & 
-    Forward_simulation_inj_exposed.Forward_simulation_inject csemS csemT ge1 ge2
-    entry_points core_data match_state core_ord}}}.
-Proof.
-intros until entry_points; intros []; intros.
-solve[eexists; eexists; eexists;
- eapply @Forward_simulation_inj_exposed.Build_Forward_simulation_inject; eauto].
-Qed.
-
-Lemma forall_inject_val_list_inject: 
-  forall j args args' (H:Forall2 (val_inject j) args args' ), 
-    val_list_inject j args args'.
-Proof.
-intros j args.
-induction args; intros;  inv H; constructor; eauto.
-Qed. 
-
-Lemma val_list_inject_forall_inject: 
-  forall j args args' (H:val_list_inject j args args'), 
-    Forall2 (val_inject j) args args' .
-Proof.
-intros j args.
-induction args; intros;  inv H; constructor; eauto.
-Qed. 
-
-Lemma forall_lessdef_val_listless: 
-  forall args args' (H: Forall2 Val.lessdef args args'), 
-    Val.lessdef_list args args' .
-Proof.
-intros args.
-induction args; intros;  inv H; constructor; eauto.
-Qed. 
-
-Lemma val_listless_forall_lessdef: 
-  forall args args' (H:Val.lessdef_list args args'), 
-    Forall2 Val.lessdef args args' .
-Proof.
-intros args.
-induction args; intros;  inv H; constructor; eauto.
-Qed. 
-
-Module CompilerCorrectness.
-
-Definition globvar_eq {V1 V2: Type} (v1:globvar V1) (v2:globvar V2) :=
-  match v1, v2 with 
-  | mkglobvar _ init1 readonly1 volatile1, 
-    mkglobvar _ init2 readonly2 volatile2 =>
-    init1 = init2 /\ readonly1 =  readonly2 /\ volatile1 = volatile2
-  end.
-
-Inductive external_description :=
-| extern_func: signature -> external_description
-| extern_globvar: external_description.
-
-Definition entryPts_ok  {F1 V1 F2 V2:Type} 
-  (P1 : AST.program F1 V1)    (P2 : AST.program F2 V2) 
-  (ExternIdents: list (ident * external_description)) 
-  (entryPts: list (val * val * signature)): Prop :=
-  forall e d, In (e,d) ExternIdents ->
-    exists b, Genv.find_symbol  (Genv.globalenv P1) e = Some b /\
-      Genv.find_symbol (Genv.globalenv P2) e = Some b /\
-      match d with
-        extern_func sig => In (Vptr b Int.zero,Vptr b Int.zero, sig) entryPts /\
-        exists f1, exists f2, Genv.find_funct_ptr (Genv.globalenv P1) b = Some f1 /\ 
-          Genv.find_funct_ptr (Genv.globalenv P2) b = Some f2
-        | extern_globvar  => exists v1, exists v2, 
-          Genv.find_var_info (Genv.globalenv P1) b = Some v1 /\
-          Genv.find_var_info (Genv.globalenv P2) b = Some v2 /\
-          globvar_eq v1 v2
-      end.
-
-Definition entryPts_inject_ok {F1 V1 F2 V2:Type} 
-  (P1 : AST.program F1 V1) (P2 : AST.program F2 V2) (j: meminj)
-  (ExternIdents : list (ident * external_description)) 
-  (entryPts: list (val * val * signature)): Prop :=
-  forall e d, In (e,d) ExternIdents ->
-    exists b1, exists b2, Genv.find_symbol (Genv.globalenv P1) e = Some b1 /\
-      Genv.find_symbol (Genv.globalenv P2) e = Some b2 /\
-      j b1 = Some(b2,0) /\
-      match d with
-      | extern_func sig => 
-        In (Vptr b1 Int.zero,Vptr b2 Int.zero, sig) entryPts /\
-        exists f1, exists f2, 
-          Genv.find_funct_ptr (Genv.globalenv P1) b1 = Some f1 /\ 
-          Genv.find_funct_ptr (Genv.globalenv P2) b2 = Some f2
-      | extern_globvar => 
-        exists v1, exists v2,
-          Genv.find_var_info  (Genv.globalenv P1) b1 = Some v1 /\
-          Genv.find_var_info  (Genv.globalenv P2) b2 = Some v2 /\
-          globvar_eq v1 v2
-      end.
-
-Definition externvars_ok  {F1 V1:Type}  (P1 : AST.program F1 V1) 
-  (ExternIdents : list (ident * external_description)) : Prop :=
-  forall b v, Genv.find_var_info  (Genv.globalenv P1) b = Some v -> 
-    exists e, Genv.find_symbol (Genv.globalenv P1) e = Some b /\ 
-      In (e,extern_globvar) ExternIdents.
-
-Definition GenvHyp {F1 V1 F2 V2} 
-  (P1 : AST.program F1 V1) (P2 : AST.program F2 V2): Prop :=
-  (forall id : ident,
-    Genv.find_symbol (Genv.globalenv P2) id =
-    Genv.find_symbol (Genv.globalenv P1) id) /\
-  (forall b : block,
-    block_is_volatile (Genv.globalenv P2) b =
-    block_is_volatile (Genv.globalenv P1) b).
-
-Inductive core_correctness (I: forall F C V  
-  (Sem : CoreSemantics (Genv.t F V) C mem) 
-  (P : AST.program F V),Prop)
-  (ExternIdents: list (ident * external_description)):
-  forall (F1 C1 V1 F2 C2 V2:Type)
-    (Sem1 : CoreSemantics (Genv.t F1 V1) C1 mem)
-    (Sem2 : CoreSemantics (Genv.t F2 V2) C2 mem)
-    (P1 : AST.program F1 V1)
-    (P2 : AST.program F2 V2), Type :=
-    corec_eq : forall  (F1 C1 V1 F2 C2 V2:Type)
-      (Sem1 : CoreSemantics (Genv.t F1 V1) C1 mem)
-      (Sem2 : CoreSemantics (Genv.t F2 V2) C2 mem)
-      (P1 : AST.program F1 V1)
-      (P2 : AST.program F2 V2)
-      (Eq_init : forall m1 : mem,
-            Genv.init_mem P1 = Some m1 -> Genv.init_mem P2 = Some m1)
-      (*(Eq_init: forall m1, initial_mem Sem1  (Genv.globalenv P1)  m1 P1.(prog_defs)->
-        (exists m2, initial_mem Sem2  (Genv.globalenv P2)  m2 P2.(prog_defs)
-          /\ m1 = m2))*)
-      entrypoints
-      (ePts_ok: entryPts_ok P1 P2 ExternIdents entrypoints)
-      (R:Forward_simulation_eq.Forward_simulation_equals mem Sem1 Sem2 
-        (Genv.globalenv P1) (Genv.globalenv P2) entrypoints), 
-      prog_main P1 = prog_main P2 -> 
-      (*HERE IS THE INJECTION OF THE GENV-ASSUMPTIONS INTO THE PROOF:*)
-      GenvHyp P1 P2 ->
-      I _ _ _  Sem1 P1 -> I _ _ _  Sem2 P2 -> 
-      core_correctness I ExternIdents F1 C1 V1 F2 C2 V2 Sem1 Sem2 P1 P2
-| corec_ext: forall (F1 C1 V1 F2 C2 V2:Type)
-  (Sem1 : RelyGuaranteeSemantics (Genv.t F1 V1) C1)
-  (Sem2 : RelyGuaranteeSemantics (Genv.t F2 V2) C2)
-  (P1 : AST.program F1 V1)
-  (P2 : AST.program F2 V2)
-  (Extends_init : forall m1 : mem, Genv.init_mem P1 = Some m1 -> 
-    exists m2, Genv.init_mem P2 = Some m2 /\ Mem.extends m1 m2)
-  (*(Extends_init: forall m1, initial_mem Sem1  (Genv.globalenv P1)  m1 P1.(prog_defs)->
-    (exists m2, initial_mem Sem2  (Genv.globalenv P2)  m2 P2.(prog_defs) 
-      /\ Mem.extends m1 m2))*)
-  entrypoints
-  (ePts_ok: entryPts_ok P1 P2 ExternIdents entrypoints)
-  (R:Forward_simulation_ext.Forward_simulation_extends Sem1 Sem2 
-    (Genv.globalenv P1) (Genv.globalenv P2) entrypoints),
-  prog_main P1 = prog_main P2 -> 
-  (*HERE IS THE INJECTION OF THE GENV-ASSUMPTIONS INTO THE PROOF:*)
-  GenvHyp P1 P2 ->
-  I _ _ _ Sem1 P1 -> I _ _ _ Sem2 P2 -> 
-  core_correctness I ExternIdents F1 C1 V1 F2 C2 V2 Sem1 Sem2 P1 P2
-
-| corec_inj : forall (F1 C1 V1 F2 C2 V2:Type)
-  (Sem1 : RelyGuaranteeSemantics (Genv.t F1 V1) C1)
-  (Sem2 : RelyGuaranteeSemantics (Genv.t F2 V2) C2)
-  (P1 : AST.program F1 V1)
-  (P2 : AST.program F2 V2)
-  entrypoints jInit
-  (Inj_init : forall m1 : mem, Genv.init_mem P1 = Some m1 -> 
-      exists m2, Genv.init_mem P2 = Some m2 /\ Mem.inject jInit m1 m2)
-  (*(Inj_init: forall m1, initial_mem Sem1  (Genv.globalenv P1)  m1 P1.(prog_defs)->
-    (exists m2, initial_mem Sem2  (Genv.globalenv P2)  m2 P2.(prog_defs)
-      /\ Mem.inject jInit m1 m2))*)
-  (ePts_ok: entryPts_inject_ok P1 P2 jInit ExternIdents entrypoints)
-  (preserves_globals: meminj_preserves_globals (Genv.globalenv P1) jInit)
-  (R:Forward_simulation_inj.Forward_simulation_inject Sem1 Sem2 
-    (Genv.globalenv P1) (Genv.globalenv P2) entrypoints),
-  prog_main P1 = prog_main P2 ->
- (*HERE IS THE INJECTION OF THE GENV-ASSUMPTIONS INTO THE PROOF:*)
-  GenvHyp P1 P2 ->
-  externvars_ok P1 ExternIdents ->
-  I _ _ _ Sem1 P1 -> I _ _ _ Sem2 P2 -> 
-  core_correctness I ExternIdents F1 C1 V1 F2 C2 V2 Sem1 Sem2 P1 P2
-
-| corec_trans: forall  (F1 C1 V1 F2 C2 V2 F3 C3 V3:Type)
-  (Sem1 : CoreSemantics (Genv.t F1 V1) C1 mem)
-  (Sem2 : CoreSemantics (Genv.t F2 V2) C2 mem)
-  (Sem3 : CoreSemantics (Genv.t F3 V3) C3 mem)
-  (P1 : AST.program F1 V1)
-  (P2 : AST.program F2 V2)
-  (P3 : AST.program F3 V3),
-  core_correctness I ExternIdents F1 C1 V1 F2 C2 V2 Sem1 Sem2 P1 P2 ->
-  core_correctness I ExternIdents F2 C2 V2 F3 C3 V3 Sem2 Sem3 P2 P3 ->
-  core_correctness I ExternIdents F1 C1 V1 F3 C3 V3 Sem1 Sem3 P1 P3.
-
-Lemma corec_I: forall {F1 C1 V1 F2 C2 V2}
-  (Sem1 : CoreSemantics (Genv.t F1 V1) C1 mem)
-  (Sem2 : CoreSemantics (Genv.t F2 V2) C2 mem)
-  (P1 : AST.program F1 V1)
-  (P2 : AST.program F2 V2)  ExternIdents I,
-  core_correctness I ExternIdents F1 C1 V1 F2 C2 V2 Sem1 Sem2 P1 P2 ->
-  I _ _ _ Sem1 P1 /\ I _ _ _ Sem2 P2.
-Proof. intros. induction X; intuition. Qed.
-
-Lemma corec_main: forall {F1 C1 V1 F2 C2 V2}
-  (Sem1 : CoreSemantics (Genv.t F1 V1) C1 mem)
-  (Sem2 : CoreSemantics (Genv.t F2 V2) C2 mem)
-  (P1 : AST.program F1 V1)
-  (P2 : AST.program F2 V2)  ExternIdents I,
-  core_correctness I ExternIdents F1 C1 V1 F2 C2 V2 Sem1 Sem2 P1 P2 ->
-  prog_main P1 = prog_main P2.
-Proof. intros. induction X; intuition. congruence. Qed.
-
-(*TRANSITIVITY OF THE GENV-ASSUMPTIONS:*)
-Lemma corec_Genv:forall {F1 C1 V1 F2 C2 V2}
-  (Sem1 : CoreSemantics (Genv.t F1 V1) C1 mem)
-  (Sem2 : CoreSemantics (Genv.t F2 V2) C2 mem)
-  (P1 : AST.program F1 V1)
-  (P2 : AST.program F2 V2)  ExternIdents I,
-  core_correctness I ExternIdents F1 C1 V1 F2 C2 V2 Sem1 Sem2 P1 P2 ->
-  GenvHyp P1 P2.
-Proof. 
-  intros. induction X; intuition. 
-  destruct IHX1.
-  destruct IHX2.
-  split; intros; eauto. rewrite H1. apply H. 
-Qed.
-
-Inductive cc_sim (I: forall F C V 
-          (Sem : RelyGuaranteeSemantics (Genv.t F V) C)
-          (P : AST.program F V), Prop)
-(ExternIdents: list (ident * external_description)) entrypoints:
-forall (F1 C1 V1 F2 C2 V2:Type)
-  (Sem1 : RelyGuaranteeSemantics (Genv.t F1 V1) C1)
-  (Sem2 : RelyGuaranteeSemantics (Genv.t F2 V2) C2)
-  (P1 : AST.program F1 V1)
-  (P2 : AST.program F2 V2), Type :=
-  ccs_eq : forall  (F1 C1 V1 F2 C2 V2:Type)
-    (Sem1 : RelyGuaranteeSemantics (Genv.t F1 V1) C1)
-    (Sem2 : RelyGuaranteeSemantics (Genv.t F2 V2) C2)
-    (P1 : AST.program F1 V1)
-    (P2 : AST.program F2 V2)
-    (Eq_init : forall m1 : mem, Genv.init_mem P1 = Some m1 -> 
-                                Genv.init_mem P2 = Some m1)
-    (*(Eq_init: forall m1, initial_mem Sem1  (Genv.globalenv P1)  m1 P1.(prog_defs)->
-      (exists m2, initial_mem Sem2 (Genv.globalenv P2)  m2 P2.(prog_defs) /\ m1=m2))*)
-    (ePts_ok: entryPts_ok P1 P2 ExternIdents entrypoints)
-    (R:Forward_simulation_eq.Forward_simulation_equals mem Sem1 Sem2 
-      (Genv.globalenv P1) (Genv.globalenv P2)  entrypoints), 
-    prog_main P1 = prog_main P2 -> 
-   (*HERE IS THE INJECTION OF THE GENV-ASSUMPTIONS INTO THE PROOF:*)
-    GenvHyp P1 P2 ->
-    I _ _ _  Sem1 P1 -> I _ _ _  Sem2 P2 -> 
-    cc_sim I ExternIdents  entrypoints F1 C1 V1 F2 C2 V2 Sem1 Sem2 P1 P2
- | ccs_ext : forall  (F1 C1 V1 F2 C2 V2:Type)
-   (Sem1 : RelyGuaranteeSemantics (Genv.t F1 V1) C1)
-   (Sem2 : RelyGuaranteeSemantics (Genv.t F2 V2) C2)
-   (P1 : AST.program F1 V1)
-   (P2 : AST.program F2 V2)
-   (Ext_init : forall m1 : mem, Genv.init_mem P1 = Some m1 -> 
-         exists m2, Genv.init_mem P2 = Some m2 /\ Mem.extends m1 m2)
-   (*(Extends_init: forall m1, initial_mem Sem1  (Genv.globalenv P1)  m1 P1.(prog_defs)->
-     (exists m2, initial_mem Sem2  (Genv.globalenv P2)  m2 P2.(prog_defs) /\
-       Mem.extends m1 m2))*)
-   (ePts_ok: entryPts_ok P1 P2 ExternIdents entrypoints)
-   (R:Coop_forward_simulation_ext.Forward_simulation_extends Sem1 Sem2 
-     (Genv.globalenv P1) (Genv.globalenv P2)  entrypoints),
-   prog_main P1 = prog_main P2 -> 
-  (*HERE IS THE INJECTION OF THE GENV-ASSUMPTIONS INTO THE PROOF:*)
-   GenvHyp P1 P2 ->
-   I _ _ _ Sem1 P1 -> I _ _ _ Sem2 P2 -> 
-               cc_sim I ExternIdents  entrypoints F1 C1 V1 F2 C2 V2 Sem1 Sem2 P1 P2
- | ccs_inj : forall  (F1 C1 V1 F2 C2 V2:Type)
-   (Sem1 : RelyGuaranteeSemantics (Genv.t F1 V1) C1)
-   (Sem2 : RelyGuaranteeSemantics (Genv.t F2 V2) C2)
-   (P1 : AST.program F1 V1)
-   (P2 : AST.program F2 V2)
-   jInit
-   (Inj_init : forall m1 : mem, Genv.init_mem P1 = Some m1 -> 
-      exists m2, Genv.init_mem P2 = Some m2 /\ Mem.inject jInit m1 m2)
-   (*(Inj_init: forall m1, initial_mem Sem1  (Genv.globalenv P1)  m1 P1.(prog_defs)->
-     (exists m2, initial_mem Sem2  (Genv.globalenv P2)  m2 P2.(prog_defs)
-       /\ Mem.inject jInit m1 m2))*)
-   (ePts_ok: entryPts_inject_ok P1 P2 jInit ExternIdents entrypoints)
-   (preserves_globals: meminj_preserves_globals (Genv.globalenv P1) jInit)
-   (R:Coop_forward_simulation_inj.Forward_simulation_inject Sem1 Sem2 
-     (Genv.globalenv P1) (Genv.globalenv P2)  entrypoints),
-   prog_main P1 = prog_main P2 ->
-   (*HERE IS THE INJECTION OF THE GENV-ASSUMPTIONS INTO THE PROOF:*)
-   GenvHyp P1 P2 ->
-   externvars_ok P1 ExternIdents ->
-   I _ _ _ Sem1 P1 -> I _ _ _ Sem2 P2 -> 
-   cc_sim I ExternIdents entrypoints  F1 C1 V1 F2 C2 V2 Sem1 Sem2 P1 P2.
-
-End CompilerCorrectness.
+End Forward_simulation.
