sepcomp/rg_forward_simulations_lemmas.v
@@ -1,0 +1,357 @@
+Require Import Coqlib.
+Require Import ListSet.
+Require Import Events.
+Require Import Memory.
+Require Import Coqlib.
+Require Import compcert.common.Values.
+Require Import AST.
+Require Import Globalenvs.
+
+Require Import sepcomp.mem_lemmas.
+Require Import sepcomp.core_semantics.
+Require Import sepcomp.rg_semantics.
+Require Import sepcomp.forward_simulations.
+Require Import sepcomp.rg_forward_simulations.
+
+
+Section Sim_EXT_SIMU_DIAGRAMS.
+  Context {G1 C1 G2 C2:Type}
+          {Sem1 : RelyGuaranteeSemantics G1 C1}
+          {Sem2 : RelyGuaranteeSemantics G2 C2}
+
+          {ge1:G1}
+          {ge2:G2}
+          {entry_points : list (val * val * signature)}.
+
+  Let core_data := C1.
+
+  Variable match_states: core_data -> C1 -> mem -> C2 -> mem -> Prop.
+
+  Hypothesis match_initial_cores: forall v1 v2 sig,
+      In (v1,v2,sig) entry_points ->
+        forall vals vals' m1 m2,
+          Forall2 Val.lessdef vals vals' ->
+          Forall2 (Val.has_type) vals' (sig_args sig) ->
+          Mem.extends m1 m2 ->
+          exists c1, exists c2,
+            initial_core Sem1 ge1 v1 vals = Some c1 /\
+            initial_core Sem2 ge2 v2 vals' = Some c2 /\
+            match_states c1 c1 m1 c2 m2.
+
+  Hypothesis ext_halted:
+      forall cd st1 m1 st2 m2 v1,
+        match_states cd st1 m1 st2 m2 ->
+        halted Sem1 st1 = Some v1 ->
+        exists v2, Val.lessdef v1 v2 /\
+            halted Sem2 st2 = Some v2 /\
+            Mem.extends m1 m2.
+
+  Hypothesis ext_at_external: 
+        forall d st1 m1 st2 m2 e vals1 sig,
+          (d = st1 /\ match_states d st1 m1 st2 m2) ->
+         at_external Sem1 st1 = Some (e, sig, vals1) ->
+         exists vals2,
+          Mem.extends m1 m2 /\
+          Forall2 Val.lessdef vals1 vals2 /\
+          Forall2 (Val.has_type) vals2 (sig_args sig) /\
+          at_external Sem2 st2 = Some (e,sig,vals2).
+
+  Hypothesis ext_after_external:
+      forall d st1 st2 m1 m2 e vals1 vals2 ret1 ret2 m1' m2' sig,
+        (d=st1 /\ match_states d st1 m1 st2 m2) ->
+        at_external Sem1 st1 = Some (e,sig,vals1) ->
+        at_external Sem2 st2 = Some (e,sig,vals2) ->
+
+        Forall2 Val.lessdef vals1 vals2 ->
+        Forall2 (Val.has_type) vals2 (sig_args sig) ->
+        mem_forward m1 m1' ->
+        mem_forward m2 m2' ->
+
+        Mem.unchanged_on (fun b ofs => 
+          loc_out_of_bounds m1 b ofs /\ private_block Sem1 st1 b) m2 m2' -> 
+       (*ie spill-locations didn't change*)        
+        Val.lessdef ret1 ret2 ->
+        Mem.extends m1' m2' ->
+
+        Val.has_type ret2 (proj_sig_res sig) ->
+
+        exists st1', exists st2', exists d',
+          after_external Sem1 (Some ret1) st1 = Some st1' /\
+          after_external Sem2 (Some ret2) st2 = Some st2' /\
+          d' = st1' /\ match_states d' st1' m1' st2' m2'. 
+
+Section EXT_SIMULATION_STAR_WF.
+Variable order: C1 -> C1 -> Prop.
+Hypothesis order_wf: well_founded order.
+
+Hypothesis ext_simulation:
+  forall c1 m1 c1' m1',  corestep Sem1 ge1 c1 m1 c1' m1' ->
+    forall c2 m2, match_states c1 c1 m1 c2 m2 ->
+      exists c2', exists m2', 
+        match_states c1' c1' m1' c2' m2' /\
+        Mem.unchanged_on (fun b ofs => 
+          loc_out_of_bounds m1 b ofs /\ ~private_block Sem1 c1 b) m2 m2' /\
+        (corestep_plus Sem2 ge2  c2 m2 c2' m2' \/ 
+          (corestep_star Sem2 ge2 c2 m2 c2' m2' /\ order c1' c1)).
+
+Lemma ext_simulation_star_wf: 
+  RGForward_simulation_ext.RGForward_simulation_extends Sem1 Sem2 ge1 ge2 entry_points.
+Proof.
+  eapply RGForward_simulation_ext.Build_RGForward_simulation_extends with
+        (core_ord := order)
+        (match_state := fun d c1 m1 c2 m2 => d = c1 /\ match_states d c1 m1 c2 m2).
+   apply order_wf.
+   intros. destruct H0; subst.
+              destruct (ext_simulation _ _ _ _ H _ _ H1) as [c2' [m2' [MC' Step]]].
+              exists c2'. exists m2'. exists st1'.  split; eauto.
+   intros. destruct (match_initial_cores _ _ _ H _ _ _ _ H0 H1 H2) 
+    as [c1' [c2' [MIC1 [MIC2 MC]]]].
+                 exists c1'. exists c1'. exists c2'. split; eauto.
+   intros. destruct H; subst. eapply ext_halted; eauto.
+   intros.  destruct H. eapply ext_at_external; eauto.
+   intros. destruct H. eapply ext_after_external; eauto.
+Qed.
+
+End EXT_SIMULATION_STAR_WF.
+
+Section EXT_SIMULATION_STAR.
+  Variable measure: C1 -> nat.
+  
+  Hypothesis ext_star_simulation:
+    forall (c1 : C1) (m1 : mem) (c1' : C1) (m1' : mem),
+      corestep Sem1 ge1 c1 m1 c1' m1' ->
+      forall (c2 : C2) (m2 : mem),
+        match_states c1 c1 m1 c2 m2 ->
+        exists c2' : C2,
+          exists m2' : mem,
+            match_states c1' c1' m1' c2' m2' /\
+            Mem.unchanged_on
+            (fun (b : block) (ofs : Z) =>
+              loc_out_of_bounds m1 b ofs /\ ~ private_block Sem1 c1 b) m2 m2' /\
+            (corestep_plus Sem2 ge2 c2 m2 c2' m2' \/ 
+             corestep_star Sem2 ge2 c2 m2 c2' m2' /\ ltof C1 measure c1' c1).
+
+Lemma ext_simulation_star: 
+  RGForward_simulation_ext.RGForward_simulation_extends Sem1 Sem2 ge1 ge2 entry_points.
+Proof.
+  eapply ext_simulation_star_wf.
+  apply  (well_founded_ltof _ measure).
+  intros.
+  destruct (ext_star_simulation _ _ _ _ H _ _ H0) as [c2' [m2' [CSP [? MC']]]].
+  exists c2'; exists m2'; split; auto.
+Qed.
+
+End EXT_SIMULATION_STAR.
+
+Section EXT_SIMULATION_PLUS.
+  Variable measure: C1 -> nat. 
+  Hypothesis ext_plus_simulation:
+    forall c1 m1 c1' m1', corestep Sem1 ge1 c1 m1 c1' m1'  -> 
+    forall c2 m2, match_states c1 c1 m1 c2 m2 ->
+      exists c2', exists m2', 
+        corestep_plus Sem2 ge2 c2 m2 c2' m2' /\ 
+        match_states c1' c1' m1' c2' m2' /\
+        Mem.unchanged_on
+        (fun (b : block) (ofs : Z) =>
+          loc_out_of_bounds m1 b ofs /\ ~ private_block Sem1 c1 b) m2 m2'.
+
+Lemma ext_simulation_plus: 
+  RGForward_simulation_ext.RGForward_simulation_extends Sem1 Sem2 ge1 ge2 entry_points.
+Proof.
+  apply ext_simulation_star with (measure:=measure).
+  intros. destruct (ext_plus_simulation _ _ _ _ H _ _ H0) as [c2' [m2' [MC [UNC STEP]]]].
+  eexists; eexists; split; eauto.
+Qed.
+
+End EXT_SIMULATION_PLUS.
+
+End Sim_EXT_SIMU_DIAGRAMS.
+
+
+Section Sim_INJ_SIMU_DIAGRAMS.
+  Context {F1 V1 C1 G2 C2:Type}
+          {Sem1 : RelyGuaranteeSemantics (Genv.t F1 V1) C1}
+          {Sem2 : RelyGuaranteeSemantics G2 C2}
+
+          {ge1: Genv.t F1 V1} 
+          {ge2:G2}
+          {entry_points : list (val * val * signature)}. 
+
+  Let core_data := C1.
+
+  Variable match_states: core_data -> meminj -> C1 -> mem -> C2 -> mem -> Prop.
+
+  Hypothesis match_initial_cores: forall v1 v2 sig,
+        In (v1,v2,sig) entry_points -> 
+       forall vals1 c1 m1 j vals2 m2,
+          initial_core Sem1 ge1 v1 vals1 = Some c1 ->
+          Mem.inject j m1 m2 -> 
+          (*Is this line needed?? 
+             (forall w1 w2 sigg,  In (w1,w2,sigg) entry_points -> val_inject j w1 w2) ->*)
+          Forall2 (val_inject j) vals1 vals2 ->
+
+          Forall2 (Val.has_type) vals2 (sig_args sig) ->
+          exists c2, 
+            initial_core Sem2 ge2 v2 vals2 = Some c2 /\
+            match_states c1 j c1 m1 c2 m2. 
+
+  Hypothesis inj_halted:forall cd j c1 m1 c2 m2 v1 rty,
+      match_states cd j c1 m1 c2 m2 ->
+      halted Sem1 c1 = Some v1 ->
+      Val.has_type v1 rty -> 
+      exists v2, val_inject j v1 v2 /\ 
+        halted Sem2 c2 = Some v2 /\
+        Val.has_type v2 rty /\
+        Mem.inject j m1 m2.
+
+  Hypothesis inj_at_external: 
+      forall d j st1 m1 st2 m2 e vals1 sig,
+        d = st1 /\ match_states d j st1 m1 st2 m2 ->
+        at_external Sem1 st1 = Some (e,sig,vals1) ->
+        ( Mem.inject j m1 m2 /\
+          meminj_preserves_globals ge1 j /\ (*LENB: also added meminj_preserves_global HERE*)
+          exists vals2, Forall2 (val_inject j) vals1 vals2 /\
+          Forall2 (Val.has_type) vals2 (sig_args (ef_sig e)) /\
+          at_external Sem2 st2 = Some (e,sig,vals2)).
+
+  Hypothesis inj_after_external:
+      forall d j j' st1 st2 m1 e vals1 (*vals2*) ret1 m1' m2 m2' ret2 sig c1 c2,
+        (d=st1 /\ match_states d j st1 m1 st2 m2) ->
+        at_external Sem1 st1 = Some (e,sig,vals1) ->
+
+    (* LENB: we may want to add meminj_preserves_globals ge1 j as another
+      asumption here, to get rid of
+      meminj_preserved_globals_inject_incr below. But this would
+      require spaeicaliing G1 to Genv.t....  Maybe we can specialize
+      G1 and G2 of CompCertCoreSem's to Genv F1 V1/Genv F2 V2, but not
+      specialize CoreSem's?*)
+
+        meminj_preserves_globals ge1 j -> 
+
+        inject_incr j j' ->
+        inject_separated j j' m1 m2 ->
+        Mem.inject j' m1' m2' ->
+        val_inject_opt j' ret1 ret2 ->
+
+         mem_forward m1 m1'  -> 
+         Mem.unchanged_on (fun b ofs => 
+           loc_unmapped j b ofs /\ private_block Sem1 c1 b) m1 m1' ->
+         mem_forward m2 m2' -> 
+         Mem.unchanged_on (fun b ofs => 
+           loc_out_of_reach j m1 b ofs /\ private_block Sem2 c2 b) m2 m2' ->
+         val_has_type_opt' ret1 (proj_sig_res (ef_sig e)) ->
+         val_has_type_opt' ret2 (proj_sig_res (ef_sig e)) ->
+
+      exists st1', exists st2', exists d',
+          after_external Sem1 ret1 st1 = Some st1' /\
+          after_external Sem2 ret2 st2 = Some st2' /\
+          d' = st1' /\ match_states d' j' st1' m1' st2' m2'. 
+
+Section INJ_SIMULATION_STAR_WF.
+Variable order: C1 -> C1 -> Prop.
+Hypothesis order_wf: well_founded order.
+
+  Hypothesis inj_simulation:
+     forall c1 m1 c1' m1',  corestep Sem1 ge1 c1 m1 c1' m1' ->
+     forall j c2 m2, match_states c1 j c1 m1 c2 m2 ->
+      exists c2', exists m2', exists j', 
+        inject_incr j j' /\
+        inject_separated j j' m1 m2 /\
+        match_states c1' j' c1' m1' c2' m2' /\
+        Mem.unchanged_on
+        (fun (b : block) (ofs : Z) =>
+          loc_unmapped j b ofs /\ ~ private_block Sem1 c1 b) m1 m1' /\
+        Mem.unchanged_on
+        (fun (b : block) (ofs : Z) =>
+          loc_out_of_reach j m1 b ofs /\ ~ private_block Sem2 c2 b) m2 m2' /\
+        (corestep_plus Sem2 ge2  c2 m2 c2' m2' \/ 
+          (corestep_star Sem2 ge2 c2 m2 c2' m2' /\ order c1' c1)).
+
+Lemma  inj_simulation_star_wf: 
+  RGForward_simulation_inj.RGForward_simulation_inject Sem1 Sem2 ge1 ge2 entry_points.
+Proof.
+  eapply RGForward_simulation_inj.Build_RGForward_simulation_inject with
+    (core_ord := order)
+    (match_state := fun d j c1 m1 c2 m2 => d = c1 /\ match_states d j c1 m1 c2 m2).
+  apply order_wf.
+  intros. destruct H0; subst.
+  destruct (inj_simulation _ _ _ _ H _ _ _ H1) as 
+    [c2' [m2' [j' [INC [SEP [MC' [UNCH1 [UNCH2 Step]]]]]]]].
+  exists c2'. exists m2'. exists st1'. exists j'. split; auto. 
+  intros. destruct (match_initial_cores _ _ _ H _ _ _ _ _ _ H0 H1 H2 H3) as 
+    [c2' [MIC MC]].
+  exists c1.  exists c2'. split; eauto.
+  intros. destruct H; subst. eapply inj_halted; eauto.
+  intros.  destruct H; subst. eapply inj_at_external; eauto.
+  intros.  (*destruct H0; subst.*) clear inj_simulation .
+  specialize (inj_after_external _ _ _ _ _ _ _ _ _ _ _ _ _ _ _ _ 
+    H0 H1 H2 H3 H4 H5 H6 H7 H8 H9 H10 H11 H12).
+  destruct inj_after_external as [c1' [c2' [d' [X1 [X2 [X3 X4]]]]]]. subst.
+  exists c1'. exists c1'. exists c2'. split; auto.
+Qed.
+
+End INJ_SIMULATION_STAR_WF.
+
+Section INJ_SIMULATION_STAR.
+  Variable measure: C1 -> nat.
+  
+  Hypothesis inj_star_simulation:
+    forall c1 m1 c1' m1', corestep Sem1 ge1 c1 m1 c1' m1'  -> 
+    forall c2 m2 j, match_states c1 j c1 m1 c2 m2 ->
+      (exists c2', exists m2', exists j', 
+        inject_incr j j' /\
+        inject_separated j j' m1 m2 /\ 
+        Mem.unchanged_on
+        (fun (b : block) (ofs : Z) =>
+          loc_unmapped j b ofs /\ ~ private_block Sem1 c1 b) m1 m1' /\
+        Mem.unchanged_on
+        (fun (b : block) (ofs : Z) =>
+          loc_out_of_reach j m1 b ofs /\ ~ private_block Sem2 c2 b) m2 m2' /\
+        match_states c1' j' c1' m1' c2' m2' /\
+        (corestep_plus Sem2 ge2 c2 m2 c2' m2' 
+          \/ ((measure c1' < measure c1)%nat /\ corestep_star Sem2 ge2 c2 m2 c2' m2'))).
+
+Lemma inj_simulation_star: 
+  RGForward_simulation_inj.RGForward_simulation_inject Sem1 Sem2 ge1 ge2 entry_points.
+Proof.
+  eapply inj_simulation_star_wf.
+  apply  (well_founded_ltof _ measure).
+  intros. destruct (inj_star_simulation _ _ _ _ H _ _ _ H0) as [c2' H1].
+  destruct H1 as [m2' [j' [INC [SEP [UNCH1 [UNCH2 [MC' STEP]]]]]]]. 
+  exists c2'. exists m2'. exists j'. split; trivial. split; trivial. split; trivial. 
+  split; auto. split; auto.
+  destruct STEP as [X1|X1]; subst. left; auto. 
+  right. destruct X1. split; auto.
+Qed.
+
+End INJ_SIMULATION_STAR.
+
+Section INJ_SIMULATION_PLUS.
+  Variable measure: C1 -> nat. 
+  Hypothesis inj_plus_simulation:
+    forall c1 m1 c1' m1', corestep Sem1 ge1 c1 m1 c1' m1'  -> 
+    forall c2 m2 j, match_states c1 j c1 m1 c2 m2 ->
+      exists c2', exists m2',  exists j', 
+        inject_incr j j' /\
+        inject_separated j j' m1 m2 /\ 
+        corestep_plus Sem2 ge2 c2 m2 c2' m2' /\ 
+        match_states c1' j' c1' m1' c2' m2' /\ 
+        Mem.unchanged_on
+        (fun (b : block) (ofs : Z) =>
+          loc_unmapped j b ofs /\ ~ private_block Sem1 c1 b) m1 m1' /\
+        Mem.unchanged_on
+        (fun (b : block) (ofs : Z) =>
+          loc_out_of_reach j m1 b ofs /\ ~ private_block Sem2 c2 b) m2 m2'.
+  
+Lemma inj_simulation_plus: 
+  RGForward_simulation_inj.RGForward_simulation_inject Sem1 Sem2 ge1 ge2 entry_points.
+Proof.
+  apply inj_simulation_star with (measure:=measure).
+  intros. destruct (inj_plus_simulation _ _ _ _ H _ _ _ H0) 
+    as [? [? [? [? [? [? [? [? ?]]]]]]]].
+  do 3 eexists. split; eauto. split; eauto.
+Qed.
+
+End INJ_SIMULATION_PLUS.
+
+End Sim_INJ_SIMU_DIAGRAMS.
